move hash to V1Model.v, but I don't know why it doesn't work

core/V1ModelSpec.v
@@ -1,5 +1,6 @@
 Require Import Coq.Strings.String.
 Require Import Coq.micromega.Lia.
+Require Import Coq.ZArith.Zcomplements.
 Require Import Poulet4.P4light.Syntax.Typed.
 Require Import Poulet4.P4light.Syntax.Syntax.
 Require Import Poulet4.P4light.Syntax.Value.
@@ -131,13 +132,102 @@ Proof.
     apply in_scopes_In. now left.
 Qed.
 
+Definition BASE : Z := 0.
+Definition MAX : Z := 1024.
+
+Section CRC.
+Import Hexadecimal.
+
+Definition CRC : list bool -> list bool := Hash.compute_crc 16%nat (D8 (D0 (D0 (D5 Nil)))) zero zero true true.
+
+Definition CRC_Z (data : list bool) : Z :=
+  BASE + Z.modulo (BitArith.lbool_to_val (CRC data) 1 0) MAX.
+
+End CRC.
+
+(* A more restricted func spec, but should be sound. *)
+Definition hash_spec : func_spec :=
+  WITH,
+    PATH []
+    MOD None []
+    WITH (data : list Val) (input : list bool)
+      (_ : concat_tuple data = Some input),
+      PRE
+        (ARG [ValBaseEnumField "HashAlgorithm" "crc16";
+              ValBaseBit (to_loptbool 32 BASE);
+              eval_val_to_sval (ValBaseTuple data);
+              ValBaseBit (to_loptbool 32 MAX)]
+        (MEM []
+        (EXT [])))
+      POST
+        (ARG_RET [ValBaseBit (to_loptbool 32%N (CRC_Z input))] ValBaseNull
+        (MEM []
+        (EXT []))).
+
+
+Lemma Forall2_bit_refine_eval_val_eq:
+  forall l1 l2, Forall2 (exec_val SvalRefine.bit_refine) (map eval_val_to_sval l1) l2 ->
+           map eval_val_to_sval l1 = l2.
+Proof.
+  induction l1; simpl; intros; inv H; auto. f_equal. 2: now apply IHl1.
+  apply exec_val_eval_val_to_sval_eq in H2; auto. intros. now inv H.
+Qed.
+
+Lemma Forall2_ndetbit_eval_val_eq: forall l1 l2,
+    Forall2 (exec_val read_ndetbit) (map eval_val_to_sval l1) l2 -> l1 = l2.
+Proof.
+  induction l1; simpl; intros; inv H; auto. f_equal. 2: now apply IHl1.
+  apply sval_to_val_eval_val_to_sval_eq in H2; auto. intros. now inv H.
+Qed.
+Lemma hash_body : forall targs,
+    fundef_satisfies_spec ge (FExternal "" "hash") (TypBit 32%N :: targs) hash_spec.
+Proof.
+  intros. unfold hash_spec. simpl. split.
+  - repeat intro. red. red in H. destruct H. do 2 red in H. inv H. inv H4.
+    inv H6. inv H3. inv H5. inv H4. inv H7. inv H8. inv H5.
+    apply Members.Forall2_bit_refine_Some_same' in H2, H4. subst. inv H0. inv H7.
+    simpl in H. inv H. simpl. red. split; [|split]; auto.
+    + Opaque to_lbool. inv H4. inv H6. inv H8. inv H4. apply Forall2_ndetbit in H2.
+      inv H7. inv H6. inv H10. inv H8. inv H6. apply Forall2_ndetbit in H4. subst.
+      inv H13. inv H7. constructor. 2: constructor. unfold bound_hash_output in H4.
+      rewrite !bit_from_to_bool in H4. vm_compute in H5. inv H5.
+      apply Forall2_bit_refine_eval_val_eq in H3. subst lv'.
+      apply Forall2_ndetbit_eval_val_eq in H2. subst vs. rewrite x1 in H9. inv H9.
+      unfold CRC_Z, CRC.
+      remember (Hexadecimal.D8
+                  (Hexadecimal.D0 (Hexadecimal.D0 (Hexadecimal.D5 Hexadecimal.Nil))))
+        as D8005. remember (Hexadecimal.D0 Hexadecimal.Nil) as D00.
+      replace (BitArith.mod_bound 32 BASE) with BASE in *
+          by (unfold BASE; now vm_compute).
+      replace (BitArith.mod_bound 32 MAX) with MAX in *
+          by (unfold MAX; now vm_compute). unfold BitArith.from_lbool in H4.
+      rewrite Zlength_correct in H4. rewrite Hash.length_compute_crc in H4.
+      change (Z.to_N (Z.of_nat 16)) with 16%N in H4. rewrite N.max_id in H4.
+      rewrite N.max_l in H4 by lia.
+      unfold BitArith.modulo_mod, BitArith.plus_mod in H4.
+      rewrite BitArith.mod_bound_double_add, to_lbool_bit_mod in H4.
+      unfold to_loptbool. revert H4.
+      generalize (to_lbool 32
+                         (BASE +
+                            BitArith.lbool_to_val
+                              (Hash.compute_crc 16 D8005 D00 D00 true true input) 1 0
+                              mod MAX)). intros. inv H4. constructor.
+      rewrite ForallMap.Forall2_forall in H0. destruct H0.
+      rewrite <- ForallMap.Forall2_map_l, ForallMap.Forall2_forall. split; auto.
+      intros. specialize (H0 _ _ H2). inv H0. constructor.
+    + repeat intro. inv H. constructor.
+  - repeat intro. unfold modifies. split; only 1 : (simpl; auto). repeat intro.
+    inv H. simpl. inv H6. simpl in H. inv H. auto.
+Qed.
+
 End V1ModelSpec.
 
 #[export] Hint Extern 5 (func_modifies _ _ _ _ _) =>
   (refine (proj2 (register_read_body _ _ _ _)); reflexivity) : func_specs.
 #[export] Hint Extern 5 (func_modifies _ _ _ _ _) =>
   (refine (proj2 (register_write_body _ _ _ _)); reflexivity) : func_specs.
-
+#[export] Hint Extern 5 (func_modifies _ _ _ _ _) => (apply hash_body) : func_specs.
+#[export] Hint Extern 1 (list P4Type) => (exact (@nil _)) : func_specs.
 (*
 Several issues:
 - out of bounds for i
