examples/bloomfilter/verif.v
@@ -141,7 +141,7 @@ Definition Add_fundef := Eval compute in
 
 Definition havoc := uninit_sval_of_sval.
 
-Section CRC.
+(* Section CRC.
 Import Hexadecimal.
 
 Definition CRC : list bool -> list bool := Hash.compute_crc 16%nat (D8 (D0 (D0 (D5 Nil)))) zero zero true true.
@@ -152,7 +152,7 @@ Definition BASE : Z := 0.
 Definition MAX : Z := 1024.
 
 Definition CRC_Z (data : list bool) : Z :=
-  BASE + Z.modulo (BitArith.lbool_to_val (CRC data) 1 0) MAX.
+  BASE + Z.modulo (BitArith.lbool_to_val (CRC data) 1 0) MAX. *)
 
 Lemma CRC_range : forall data, 0 <= CRC_Z data < NUM_ENTRY.
 Proof.
@@ -185,88 +185,7 @@ Definition bloomfilter_query bf data :=
 Definition havoc_typ (typ : @P4Type Info) : Sval :=
   force ValBaseNull (uninit_sval_of_typ None typ).
 
-Definition hash_fundef :=
-  force dummy_fundef (PathMap.get ["hash"] (ge_func ge)).
-
 Open Scope arg_ret_assr.
-
-Lemma Forall2_bit_refine_eval_val_eq:
-  forall l1 l2, Forall2 (exec_val SvalRefine.bit_refine) (map eval_val_to_sval l1) l2 ->
-           map eval_val_to_sval l1 = l2.
-Proof.
-  induction l1; simpl; intros; inv H; auto. f_equal. 2: now apply IHl1.
-  apply exec_val_eval_val_to_sval_eq in H2; auto. intros. now inv H.
-Qed.
-
-Lemma Forall2_ndetbit_eval_val_eq: forall l1 l2,
-    Forall2 (exec_val read_ndetbit) (map eval_val_to_sval l1) l2 -> l1 = l2.
-Proof.
-  induction l1; simpl; intros; inv H; auto. f_equal. 2: now apply IHl1.
-  apply sval_to_val_eval_val_to_sval_eq in H2; auto. intros. now inv H.
-Qed.
-
-(* A more restricted func spec, but should be sound. *)
-Definition hash_spec : func_spec :=
-  WITH,
-    PATH []
-    MOD None []
-    WITH (data : list Val) (input : list bool)
-      (_ : concat_tuple data = Some input),
-      PRE
-        (ARG [ValBaseEnumField "HashAlgorithm" "crc16";
-              ValBaseBit (to_loptbool 32 BASE);
-              eval_val_to_sval (ValBaseTuple data);
-              ValBaseBit (to_loptbool 32 MAX)]
-        (MEM []
-        (EXT [])))
-      POST
-        (ARG_RET [ValBaseBit (to_loptbool 32%N (CRC_Z input))] ValBaseNull
-        (MEM []
-        (EXT []))).
-
-Lemma hash_body : forall targs,
-    fundef_satisfies_spec ge hash_fundef (TypBit 32%N :: targs) hash_spec.
-Proof.
-  intros. unfold hash_spec. simpl. split.
-  - repeat intro. red. red in H. destruct H. do 2 red in H. inv H. inv H4.
-    inv H6. inv H3. inv H5. inv H4. inv H7. inv H8. inv H5.
-    apply Members.Forall2_bit_refine_Some_same' in H2, H4. subst. inv H0. inv H7.
-    simpl in H. inv H. simpl. red. split; [|split]; auto.
-    + Opaque to_lbool. inv H4. inv H6. inv H8. inv H4. apply Forall2_ndetbit in H2.
-      inv H7. inv H6. inv H10. inv H8. inv H6. apply Forall2_ndetbit in H4. subst.
-      inv H13. inv H7. constructor. 2: constructor. unfold bound_hash_output in H4.
-      rewrite !bit_from_to_bool in H4. vm_compute in H5. inv H5.
-      apply Forall2_bit_refine_eval_val_eq in H3. subst lv'.
-      apply Forall2_ndetbit_eval_val_eq in H2. subst vs. rewrite x1 in H9. inv H9.
-      unfold CRC_Z, CRC.
-      remember (Hexadecimal.D8
-                  (Hexadecimal.D0 (Hexadecimal.D0 (Hexadecimal.D5 Hexadecimal.Nil))))
-        as D8005. remember (Hexadecimal.D0 Hexadecimal.Nil) as D00.
-      replace (BitArith.mod_bound 32 BASE) with BASE in *
-          by (unfold BASE; now vm_compute).
-      replace (BitArith.mod_bound 32 MAX) with MAX in *
-          by (unfold MAX; now vm_compute). unfold BitArith.from_lbool in H4.
-      rewrite Zlength_correct in H4. rewrite Hash.length_compute_crc in H4.
-      change (Z.to_N (Z.of_nat 16)) with 16%N in H4. rewrite N.max_id in H4.
-      rewrite N.max_l in H4 by lia.
-      unfold BitArith.modulo_mod, BitArith.plus_mod in H4.
-      rewrite BitArith.mod_bound_double_add, to_lbool_bit_mod in H4.
-      unfold to_loptbool. revert H4.
-      generalize (to_lbool 32
-                         (BASE +
-                            BitArith.lbool_to_val
-                              (Hash.compute_crc 16 D8005 D00 D00 true true input) 1 0
-                              mod MAX)). intros. inv H4. constructor.
-      rewrite ForallMap.Forall2_forall in H0. destruct H0.
-      rewrite <- ForallMap.Forall2_map_l, ForallMap.Forall2_forall. split; auto.
-      intros. specialize (H0 _ _ H2). inv H0. constructor.
-    + repeat intro. inv H. constructor.
-  - repeat intro. unfold modifies. split; only 1 : (simpl; auto). repeat intro.
-    inv H. simpl. inv H6. simpl in H. inv H. auto.
-Qed.
-
-#[local] Hint Extern 5 (func_modifies _ _ _ _ _) => (apply hash_body) : func_specs.
-#[local] Hint Extern 1 (list P4Type) => (exact (@nil _)) : func_specs.
 
 (*
 control Add(inout headers hdr, inout custom_metadata_t meta) {
